TermTests/CtorFnTest/Module.lean
@@ -17,9 +17,9 @@ structure Pt where
 
 def natT : TyWf := .prim .nat
 
-def green : Term ⟨[], rfl⟩ [] (#leanscript_layout `Color `green) := #leanscript_ctor `Color `green
-def pt : Term ⟨[], rfl⟩ [] (#leanscript_layout `Pt) := #leanscript_ctor `Pt (.nat_mk 1) (.nat_mk 2)
-def some3 : Term ⟨[], rfl⟩ [] (#leanscript_layout `Option `some natT) :=
+def green : Term ⟨[], List.nodup_nil⟩ [] (#leanscript_layout `Color `green) := #leanscript_ctor `Color `green
+def pt : Term ⟨[], List.nodup_nil⟩ [] (#leanscript_layout `Pt) := #leanscript_ctor `Pt (.nat_mk 1) (.nat_mk 2)
+def some3 : Term ⟨[], List.nodup_nil⟩ [] (#leanscript_layout `Option `some natT) :=
   #leanscript_ctor `Option `some natT (.nat_mk 3)
 
 end CtorFnModuleTest
